\documentclass[]{ximera}
%handout:  for handout version with no solutions or instructor notes
%handout,instructornotes:  for instructor version with just problems and notes, no solutions
%noinstructornotes:  shows only problem and solutions

%% handout
%% space
%% newpage
%% numbers
%% nooutcomes

%I added the commands here so that I would't have to keep looking them up
%\newcommand{\RR}{\mathbb R}
%\renewcommand{\d}{\,d}
%\newcommand{\dd}[2][]{\frac{d #1}{d #2}}
%\renewcommand{\l}{\ell}
%\newcommand{\ddx}{\frac{d}{dx}}
%\everymath{\displaystyle}
%\newcommand{\dfn}{\textbf}
%\newcommand{\eval}[1]{\bigg[ #1 \bigg]}

%\begin{image}
%\includegraphics[trim= 170 420 250 180]{Figure1.pdf}
%\end{image}

%add a ``.'' below when used in a specific directory.

\input{../../../preamble.tex}



\author{Tom Needham}

\outcome{Understand notation for sequences.}
\outcome{Manipulate and combine sequences defined recursively or by explicit formulas.} 

\title[]{Introduction to Sequences}

\begin{document}
\begin{abstract}
\end{abstract}
\maketitle

\vspace{-0.4in}

\section{Discussion Questions}

\begin{problem}
Classify the sequences defined by the following formulas as geometric, arithmetic or neither.
\begin{center}
\begin{tabular}{lll}
I. $a_n = 5n + 7$ \hspace{.4in} II. $b_n = n^2 + 1$ \hspace{.4in} III. $c_1 = 10, \; c_{n+1}= 2\cdot c_n$
\end{tabular}
\end{center}
\end{problem}

\begin{freeResponse}
I. The sequence $\{a_n\}$ is arithmetic, since 
$$
a_{n+1}-a_n = 5(n+1)+7-(5n+7) = 5n + 5 + 7 - 5n - 7 = 5
$$
is a constant for all $n$.

II. The sequence $\{b_n\}$ is not arithmetic, since
$$
b_{n+1}-b_n = (n+1)^2 + 1 - (n^2+1) = n^2 + 2n + 1 + 1 - n^2 - 1 = 2n + 2
$$
is not constant. It is also not geometric, since
$$
\frac{b_{n+1}}{b_n} = \frac{(n+1)^2 + 1}{n^2 + 1} = \frac{n^2+2n + 2}{n^2 + 1}
$$
is not constant.

III. The sequence $\{c_n\}$ is geometric. This is true  because, for $n\geq 1$, we have
$$
\frac{c_{n+1}}{c_n} = \frac{2 c_n}{c_n} = 2,
$$
which is constant.
\end{freeResponse}


\section{Group Work}

\begin{problem}
Let $\{a_n\}_{n=0}^\infty$ be the sequence defined by the recursive formula
$$
a_0 = 1, \; a_{n+1}=\frac{n+1}{2} \cdot a_n.
$$
Write out the first four terms of the sequence.

Let $\{b_n\}_{n=0}^\infty$ be the sequence defined by the explicit formula 
$$
b_n = \frac{n!}{2^n}.
$$
Write out the first four terms of the sequence.

You should notice that the first four terms of the sequences are the same. Show that for \emph{every} $n \geq 0$, $a_n = b_n$. 
\end{problem}

\begin{freeResponse}
The first four terms of $\{a_n\}$ are
\begin{align*}
a_0 &= 1 \\
a_1 &= \frac{1}{2} a_0 = \frac{1}{2} \\
a_2 &= \frac{2}{2} a_1 = \frac{1}{2} \\
a_3 &= \frac{3}{2} a_2 = \frac{3}{4}.
\end{align*}
The first four terms of $\{b_n\}$ are 
\begin{align*}
b_0 &= \frac{0!}{2^0} = 1\\
b_1 &= \frac{1!}{2^1} = \frac{1}{2}\\
b_2 &= \frac{2!}{2^2} = \frac{2}{4} = \frac{1}{2} \\
b_3 &= \frac{3!}{2^3} = \frac{6}{8} = \frac{3}{4}.\\
\end{align*}

To show that $a_n = b_n$ for all $n \geq 0$, we will show that the terms in $\{b_n\}$ satisfy the recursion formula defining $\{a_n\}$. We already have shown that $b_0 = 1$. Moreover, we have
$$
b_{n+1} = \frac{(n+1)!}{2^{n+1}} = \frac{(n+1) \cdot n!}{2 \cdot 2^n} = \frac{n+1}{2} \cdot \frac{n!}{2^n} = \frac{n+1}{2} b_n.
$$
\end{freeResponse}

\pagebreak

\begin{problem}
Let $\{a_n\}_{n=1}^\infty$ be the sequence given by the formula 
$$
a_n = \frac{1}{n!}
$$
Write the out the first four terms of each of sequences defined by the following formulas. Each sequence is defined for $n \geq 1$. 
\begin{center}
\begin{tabular}{lll}
I. $s_n = \sum_{j=1}^n a_j$ \hspace{.4in} II. $b_n = \frac{a_{n+1}}{a_n}$ \hspace{.4in} III. $c_n = \sqrt[n]{a_n}$
\end{tabular}
\end{center}
For the sequence defined in part II, find a simplified form for the $n$th term $b_n$. 
\end{problem}

\begin{freeResponse}
I. The first four terms of $\{s_n\}$ are 
\begin{align*}
s_1 &= a_1 = 1\\
s_2 &= a_1 + a_2 = 1 + \frac{1}{2} = \frac{3}{2}\\
s_3 &= s_2 + a_3 = \frac{3}{2} + \frac{1}{6} = \frac{5}{3} \\
s_4 &= s_3 + a_4  = \frac{5}{3} + \frac{1}{24} = \frac{41}{24}.\\
\end{align*}

II. The first four terms of $\{b_n\}$ are 
\begin{align*}
b_1 &= \frac{a_2}{a_1} = \frac{1/2}{1} = \frac{1}{2} \\
b_2 &= \frac{a_3}{a_2} = \frac{1/6}{1/2} = \frac{1}{3} \\
b_3 &= \frac{a_4}{a_3} = \frac{1/24}{1/6} = \frac{1}{4} \\
b_4 &= \frac{a_5}{a_4} = \frac{1/120}{1/24} = \frac{1}{5}.\\
\end{align*}
After looking at these terms, one might guess that $b_n = \frac{1}{n+1}$ for all $n \geq 1$. Indeed, we have
$$
b_n = \frac{a_{n+1}}{a_n} = \frac{1/(n+1)!}{1/n!} = \frac{n!}{(n+1)!} = \frac{n!}{(n+1) \cdot n!} = \frac{1}{n+1}.
$$

III. The first four terms of $\{c_n\}$ are
\begin{align*}
c_1 &= \sqrt[1]{a_1} = 1\\
c_2 &= \sqrt[2]{a_2} = \sqrt{\frac{1}{2}} \\
c_3 &= \sqrt[3]{a_3} = \sqrt[3]{\frac{1}{6}} \\
c_4 &= \sqrt[4]{a_4} = \sqrt[4]{\frac{1}{24}}.\\
\end{align*}
\end{freeResponse}

\begin{problem}
Let $\{a_n\}_{n=1}^\infty$ be the sequence defined by the formula
$$
a_n = \frac{n+2}{3^n}
$$
and let $\{b_n\}_{n=0}^\infty$ be the sequence defined recursively by
$$
b_0 = 1 \mbox{ and } b_{n+1} = b_n + \frac{1}{b_n}.
$$
Write the out the first four terms of each of sequences defined by the following formulas.
\begin{center}
\begin{tabular}{lll}
I. $\{a_n+b_n\}_{n=1}^\infty$ \hspace{.3in} II. $\{a_{n+1}/b_n\}_{n=0}^\infty$ \hspace{.3in} III. $c_1 = 1, \; c_{n+1} = c_n + a_n + b_n$
\end{tabular}
\end{center}
\end{problem}

\begin{freeResponse}
It seems that it would be useful to first write out several terms of the squences $\{a_n\}$ and $\{b_n\}$:
\begin{align*}
a_1 &= \frac{3}{3} = 1 \\
a_2 &= \frac{4}{3^2} = \frac{4}{9} \\
a_3 &= \frac{5}{3^3} = \frac{5}{27} \\
a_4 &= \frac{6}{3^4} = \frac{6}{81} = \frac{2}{27}\\
\end{align*}
and 
\begin{align*}
b_0 &= 1\\
b_1 &= 1 + \frac{1}{1} = 2\\
b_2 &= 2 + \frac{1}{2} = \frac{5}{2}\\
b_3 &= \frac{5}{2} + \frac{2}{5} = \frac{29}{10} \\
b_4 &= \frac{29}{10} + \frac{10}{29} = \frac{29^2 + 10^2}{290} = \frac{941}{290}\\
\end{align*}

I. The first four terms of the sequence $\{a_n + b_n\}_{n=1}^\infty$ are 
\begin{align*}
a_1 + b_1 &= 1 + 2 = 3\\
a_2 + b_2 &= \frac{4}{9} + \frac{5}{2}\\
a_3 + b_3 &= \frac{5}{27} + \frac{29}{10} \\
a_4 + b_4 &= \frac{2}{27} + \frac{941}{290}.\\
\end{align*}

II. The first four terms of the sequence $\{a_{n+1}/b_n\}$ are 
\begin{align*}
\frac{a_1}{b_0} &= 1 \\
\frac{a_2}{b_1} &= \frac{4/9}{2} = \frac{2}{9} \\
\frac{a_3}{b_2} &= \frac{5/27}{5/2} = \frac{2}{27}\\
\frac{a_4}{b_3} &= \frac{2/27}{29/10} = \frac{20}{783}.\\
\end{align*}

III. The first four terms of $\{c_n\}$ are 
\begin{align*}
c_1 &= 1 \\
c_2 &= c_1 + a_1 + b_1 = 1 + 3 = 4 \\
c_3 &= c_2 + a_2 + b_2 = 4 + \frac{4}{9} + \frac{5}{2} \\
c_4 &= c_3 + a_3 + b_3 =  4 + \frac{4}{9} + \frac{5}{2} + \frac{5}{27} + \frac{29}{10}\\
\end{align*}
\end{freeResponse}


\end{document}
