\documentclass[]{ximera}
%handout:  for handout version with no solutions or instructor notes
%handout,instructornotes:  for instructor version with just problems and notes, no solutions
%noinstructornotes:  shows only problem and solutions

%% handout
%% space
%% newpage
%% numbers
%% nooutcomes

%I added the commands here so that I would't have to keep looking them up
%\newcommand{\RR}{\mathbb R}
%\renewcommand{\d}{\,d}
%\newcommand{\dd}[2][]{\frac{d #1}{d #2}}
%\renewcommand{\l}{\ell}
%\newcommand{\ddx}{\frac{d}{dx}}
%\everymath{\displaystyle}
%\newcommand{\dfn}{\textbf}
%\newcommand{\eval}[1]{\bigg[ #1 \bigg]}

%\begin{image}
%\includegraphics[trim= 170 420 250 180]{Figure1.pdf}
%\end{image}

%add a ``.'' below when used in a specific directory.
\input{../../../preamble.tex} %% we can turn off input when making a master document


\title{Section 7.2: Integration By Parts}  

\begin{document}
\begin{abstract}		\end{abstract}
\author{Tom Needham}

\outcome{Apply the Integration by Parts technique to evaluate definite and indefinite integrals.}
\maketitle




\section{Discussion Questions:}


\begin{problem}
A student evaluates the integral 
$$
\int_0^1 x e^x \d x
$$
via Integration by Parts with $u=x$, $\d v = e^x \d x$ as follows:
$$
\int_0^1 x e^x \d x = x e^x - \int_0^1 e^x \d x = x e^x + \eval{e^x}_0^1 = x e^x + e^1 - e^0 = xe^x + e -1.
$$
Is the student's work correct?
\end{problem}

\begin{freeResponse}
The student's work is certainly not correct! Since they are evaluating a definite integral, their answer should be a number. However, their answer is a function of the integration variable $x$. In particular, the student forgot to evaluate the first term during the course of the integration by parts process. The correct solution is 
$$
\int_0^1 x e^x \d x = \eval{x e^x}_0^1 - \int_0^1 e^x \d x = e^1 - 0e^0 + \eval{e^x}_0^1 = e^1 + e^1 - e^0 = 2e -1.
$$
\end{freeResponse}

\begin{problem}
For each example, decide on an integration strategy (but don't actually evaluate the integrals).

\begin{center}
\begin{tabular}{lll}
I. $\int x \sin (x) \d x$ \hspace{0.2in} & II. $\int x \sin (x^2) \d x$  \hspace{0.2in} & III. $\int x^2 \sin (x) \d x$.
\end{tabular}
\end{center}
\end{problem}

\begin{freeResponse}
I. This integral is easily solved via Integration by Parts, with $u=x$ and $\d v = \sin(x) \d x$.

II. This integral can be solved via $u$-substitution with $u = x^2$, so that $\d u = 2 x \d x$.

III. Integration by Parts can be used for this example, with $u=x^2$ and $\d v = \sin(x) \d x$. After applying the method once, the integral reduces to 
$$
\int x^2 \sin (x) \d x = -x^2\cos(x) + 2\int x \cos(x) \d x.
$$
The second term can be evaluated by applying Integration by Parts once more with $u = x$ and $\d v = \cos (x) \d x$. 
\end{freeResponse}
\section{Group work:}


%problem 1
\begin{problem}
Evaluate the following integrals
\begin{center}
\begin{tabular}{lll}
I. $\int_1^3 x^2 e^{2x} \d x$ \hspace{0.2in} & II. $\int \arcsin(x) \d x$  \hspace{0.2in} & III. $\int x^{\frac{5}{3}} (\ln x)^2 \d x$.
\end{tabular}
\end{center}
\end{problem}
	
\begin{freeResponse}
I. We use Integration by Parts with $u = x^2$ and $\d v = e^{2x} \d x$, so that $\d u = 2x \d x$ and $v = \frac{1}{2} e^{2x}$. Then
$$
\int_1^3 x^2 e^{2x} \d x = \eval{\frac{x^2}{2} e^{2x}}_1^3 - \int_1^3 x e^{2x} \d x.
$$
The second integral is evaluated by another application of Integration by Parts, with $u =x$, $\d v = e^{2x} \d x$, $\d u = \d x$ and $v = \frac{1}{2}e^{2x}$. Continuing our integration, we have 
\begin{align*}
\eval{\frac{x^2}{2} e^{2x}}_1^3 - \int_1^3 x e^{2x} \d x & = \frac{9}{2} e^6 - \frac{1}{2} e^2 - \eval{\frac{x}{2}e^{2x}}_1^3 + \int_1^3 \frac{1}{2} e^{2x} \d x \\
& = \frac{9}{2} e^6 - \frac{1}{2} e^2 - \frac{3}{2} e^6 + \frac{1}{2} e^2 + \eval{\frac{1}{4}e^{2x}}_1^3 \\
& = 3e^6 + \frac{1}{4} e^6 - \frac{1}{4} e^2 \\
& = \frac{13}{4} e^6 - \frac{1}{4} e^2.
\end{align*}

II. We do not know how to integrate $\arcsin(x)$, but we do know how to differentiate it, so we will use integration by parts. Let $u = \arcsin(x)$ and $\d v =  \d x$. Then $\d u = \frac{1}{\sqrt{1-x^2}} \d x$ and $v = x$. This gives us
$$
\int \arcsin(x) \d x = x\arcsin(x) - \int \frac{x \d x}{\sqrt{1-x^2}}.
$$
The second term can be evaluated by $u$-substitution, with $u = 1- x^2$ and $\d u = -2x \d x$.  This yields
	\begin{align*}
	\int \frac{x \d x}{\sqrt{1-x^2}} &= \int \frac{-\d u}{2\sqrt{u}}\\
	&= -\frac{1}{2} \int u^{-\frac{1}{2}} \d u \\
	&= -\frac{1}{2} \cdot 2u^{\frac{1}{2}} +C \\
	&= - \sqrt{1-x^2} +C.
	\end{align*}
Therefore
$$
	\int \arcsin(x) \d x  = x\arcsin(x) + \sqrt{1-x^2} +C.
	$$
	
III. We begin with the substitution $w = \ln x$, so that $\d w = \frac{1}{x} \d x$. Solving the substitution equation for $x$ yields $x = e^w$, and we have
		\begin{align*}
		\int x^{\frac{5}{3}} (\ln x)^2 \d x 
		&= \int x^{\frac{8}{3}} (\ln x)^2 \cdot \frac{1}{x} \d x  \\
		&= \int (e^w)^{\frac{8}{3}} w^2 \d w  \\
		&= \int w^2 e^{\frac{8}{3} w} \d w.
		\end{align*}
	We now use integration by parts, with $u = w^2$ and $\d v = e^{\frac{8}{3} w} \d w$, whence $\d u = 2 w \d w$ and $v = \frac{3}{8} e^{\frac{8}{3} w}$. This gives us
		\begin{align*}
		\int x^{\frac{5}{3}} (\ln x)^2 \d x
		&= \frac{3}{8} w^2 e^{\frac{8}{3} w} - \int \frac{3}{8} (2w) e^{\frac{8}{3} w} \d w  \\
		&= \frac{3}{8} w^2 e^{\frac{8}{3} w} - \frac{3}{4} \int w e^{\frac{8}{3} w} \d w.
		\end{align*}
	To evaluate the second term, we apply integration by parts one last time with $u = w$, $\d u = \d w$, 	$\d v = e^{\frac{8}{3} w} \d w$ and $v = \frac{3}{8} e^{\frac{8}{3} w}$. This yields
		\begin{align*}
		\int x^{\frac{5}{3}} (\ln x)^2 \d x
		&= \frac{3}{8}w^2 e^{\frac{8}{3} w} - \frac{3}{4} \left( \frac{3}{8} w e^{\frac{8}{3} w} - \frac{3}{8} \int e^{\frac{8}{3} w} \d w \right) \\
		&= \frac{3}{8} w^2 e^{\frac{8}{3} w} - \frac{9}{32} w e^{\frac{8}{3} w} + \frac{27}{256} e^{\frac{8}{3} w} + C  \\
		&= \frac{3}{8} e^{\frac{8}{3} \ln x} \left( (\ln x)^2 - \frac{3}{4} \ln x + \frac{9}{32} \right) + C  \\
		&= \frac{3}{8} x^{\frac{8}{3}} \left( (\ln x)^2 - \frac{3}{4} \ln x + \frac{9}{32} \right) + C.
		\end{align*}
\end{freeResponse}





\pagebreak

%problem 2
\begin{problem}

Evaluate the following integrals

\begin{center}
\begin{tabular}{ll}
I. $\int \sin(3x) e^{7x} \d x$ \hspace{.5in} II. $\int x^5 \cos \left( x^3 \right) \d x$
\end{tabular}
\end{center}
	
\end{problem}

\begin{freeResponse}
I. We begin by letting $I = \int \sin(3x) e^{7x} \d x$.  
	We then use integration by parts with
		\[
		u = e^{7x} \qquad \d v = \sin(3x) \d x
		\]
		\[
		\d u = 7e^{7x} \d x \qquad v = -\frac{1}{3} \cos(3x).
		\]
	Then
		\begin{align*}
		I = \int \sin(3x) e^{7x} \d x &= -\frac{1}{3} e^{7x} \cos(3x) - \int -\frac{1}{3} (7e^{7x}) \cos(3x) \d x  \\
		 &= -\frac{1}{3} e^{7x} \cos(3x) + \frac{7}{3} \int e^{7x} \cos(3x) \d x.
		\end{align*}
	We then apply integration by parts again, this time with
		\[
		u = e^{7x} 		\qquad	\d v = \cos(3x) \d x
		\]
		\[
		\d u = 7e^{7x} \d x 	\qquad	v = \frac{1}{3} \sin(3x).
		\]
	This gives us
		\begin{align*}
		I &= -\frac{1}{3} e^{7x} \cos(3x) + \frac{7}{3} \left[ \frac{1}{3} e^{7x} \sin(3x) - \int \frac{1}{3} (7e^{7x}) \sin(3x) \d x \right]  \\
				&= -\frac{1}{3} e^{7x} \cos(3x) + \frac{7}{9} e^{7x} \sin(3x) - \frac{49}{9} \int e^{7x} \sin(3x) \d x  \\
		&= -\frac{1}{3} e^{7x} \cos(3x) + \frac{7}{9} e^{7x} \sin(3x) - \frac{49}{9} I.
		\end{align*}
		Since we are interested in the integral $I$, we solve the above equation for $I$ to obtain
		$$
		\frac{58}{9} I = -\frac{1}{3} e^{7x} \cos(3x) + \frac{7}{9} e^{7x} \sin(3x),
		$$
		so that 
		$$
		I = \frac{9}{58} \left( -\frac{1}{3} e^{7x} \cos(3x) + \frac{7}{9} e^{7x} \sin(3x) \right) + C.
		$$
		
		II. We begin with the substitution $w = x^3$, so that $\d w = 3x^2 \d x$. It follows that 
		\begin{align*}
		\int x^5 \cos \left( x^3 \right) \d x 
		&= \int x^3 \cos \left( x^3 \right) \cdot x^2 \d x  \\
		&= \int w \cos(w) \cdot \frac{1}{3} \d w  \\
		&= \frac{1}{3} \int w \cos(w) \d w.
		\end{align*}
	We then use integration by parts, with
		\[
		u = w 		\qquad	\d v = \cos(w) \d w
		\]
		\[
		\d u = \d w 	\qquad	v = \sin(w),
		\]
	which yields
		\begin{align*}
		\int x^5 \cos \left( x^3 \right) \d x 
		&= \frac{1}{3} \left( w \sin(w) - \int \sin(w) \d w \right)  \\
		&= \frac{1}{3} \left( w \sin(w) + \cos(w) \right) + C  \\
		&= \frac{1}{3} \left( x^3 \sin \left( x^3 \right) + \cos \left( x^3 \right) \right) + C.  
		\end{align*}
\end{freeResponse}

\begin{problem}
The region $R$ is bounded by the curves $y=0$, $y=\ln (x)$ and $x=e$. Using the shell method, find the volume of the solid formed by rotating $R$ around the $y$-axis.
\end{problem}

\begin{freeResponse}
Since we are rotating around a vertical axis and we wish to use the Shell method, our slices should be vertical. The height of the shell at $x$ is given by $\ln (x)$, and our bounds of integration are $x=1$ (corresponding to $y=0$) and $x=e$. The volume integral is 
$$
\int_1^e 2 \pi x \ln (x) \d x.
$$ 
To evaluate the integral, we use integration by parts with $u = \ln (x)$ and $\d v = x \d x$, so that $\d u = \frac{1}{x} \d x$ and $v = \frac{x^2}{2}$. This gives us 
\begin{align*}
\int_1^e 2 \pi x \ln (x) \d x &= \eval{\frac{x^2}{2} \ln x}_1^e - \int_1^e \frac{x}{2} \d x \\
&= \frac{e^2}{2}\ln(e) - \frac{1}{2}\ln (1) - \eval{\frac{x^2}{4}}_1^e \\
&= \frac{e^2}{2} - \frac{e^2}{4} + \frac{1}{4} \\
&= \frac{e^2}{4} + \frac{1}{4}.
\end{align*}
\end{freeResponse}
\end{document} 


















