\documentclass[]{ximera}
%handout:  for handout version with no solutions or instructor notes
%handout,instructornotes:  for instructor version with just problems and notes, no solutions
%noinstructornotes:  shows only problem and solutions

%% handout
%% space
%% newpage
%% numbers
%% nooutcomes

%I added the commands here so that I would't have to keep looking them up
%\newcommand{\RR}{\mathbb R}
%\renewcommand{\d}{\,d}
%\newcommand{\dd}[2][]{\frac{d #1}{d #2}}
%\renewcommand{\l}{\ell}
%\newcommand{\ddx}{\frac{d}{dx}}
%\everymath{\displaystyle}
%\newcommand{\dfn}{\textbf}
%\newcommand{\eval}[1]{\bigg[ #1 \bigg]}

%\begin{image}
%\includegraphics[trim= 170 420 250 180]{Figure1.pdf}
%\end{image}

%add a ``.'' below when used in a specific directory.

\input{../../../preamble.tex}



\author{Tom Needham}

\outcome{Use trigonometric identities to evaluate integrals.}

\title[]{Trigonometric Integrals}

\begin{document}
\begin{abstract}
\end{abstract}
\maketitle


\section{Discussion Questions}

\begin{problem}
Determine an effective strategy for evaluating each of the following integrals (you do not actually need to evaluate the integrals).

\begin{center}
\begin{tabular}{lll}
I. $\int \cos^2(x) \d x$ \hspace{.1in} & II. $\int \sin (x) \cos^2(x) \d x$ \hspace{.1in} &  III. $\int \sin^2(x) \cos^2(x) \d x$
\end{tabular}
\end{center}
\end{problem}

\begin{freeResponse}
I. This integral can be solved using the cosine half-angle identity 
$$
\cos^2(x) = \frac{1+\cos(2x)}{2},
$$
together with basic integration rules.

II. This integral can be solved via $u$-substitution, with $u=\cos (x)$, so that $\d u = -\sin (x) \d x$.

III. To solve this integral, use the double-angle identity
$$
\sin (2x) = 2 \sin(x) \cos(x),
$$
which implies
$$
\int \sin^2(x) \cos^2(x) \d x= \int \frac{1}{4} \sin^2(2x) \d x.
$$
Next we use a half-angle identity for sine, following a similar process to that used in part I.
\end{freeResponse}

\begin{problem}
Consider the integral
$$
\int \tan (x) \sec^2(x) \d x.
$$
Student A evaluates this integral by making the substitution $u=\tan(x)$, so that $\d u = \sec^2 (x)$, and
$$
\int \tan(x) \sec^2(x) \d x = \int u \d u = \frac{u^2}{2} + C = \frac{\tan^2 (x)}{2} + C.
$$
Student B makes the substitution $u = \sec(x)$, so that $\d u = \sec(x) \tan(x)$, and the integral becomes
$$
\int \tan (x) \sec^2 (x) \d x = \int \sec(x) \sec (x) \tan (x) \d x = \int u \d u = \frac{u^2}{2} +C = \frac{\sec^2(x)}{2} +C.
$$
Which of the students' solutions is correct? Either find a mistake in a student's work, or reconcile the two answers.
\end{problem}

\begin{freeResponse}
Both solutions are correct. To reconcile the answers, note that the difference between the non-constant parts of their answers is 
$$
\frac{\tan^2 (x)}{2} - \frac{\sec^2(x)}{2} = \frac{\tan^2(x) - \sec^2(x)}{2}  = -\frac{1}{2},
$$
where the last equality follows by a trigonometric identity. We conclude that the students' answers are equal, since indefinite integrals are only defined up to an additive constant.
\end{freeResponse}

\section{Group Work}

\begin{problem}
Evaluate the following integrals

\begin{center}
\begin{tabular}{llll}
I. $\displaystyle\int \sin^3 (4 \theta) \cos^6 (4\theta) \, \mathrm{d}\theta$ \hspace{.2in} & II. $\int \tan^{23} x \sec^6 x \d x$ \\
III. $\int \tan^2 x \sec x \d x$ \hspace{.2in} &  IV. $\int \tan^2 x \sin x \d x$
\end{tabular}
\end{center}
\end{problem}

\begin{freeResponse}
I. Write $\sin^3(4\theta) = \sin(4\theta) \sin^2(4\theta) = \sin(4\theta) (1-\cos^2(4\theta))$ and let $u = \cos(4\theta)$, whence $\d u = -4 \sin (4\theta) \d \theta$. The integral becomes
\begin{align*}
\int \sin^3 (4 \theta) \cos^6 (4\theta) \, \mathrm{d}\theta &= -\frac{1}{4} \int (1-u^2)u^6 \d u \\
&= -\frac{1}{4} \int (1-u^2)u^6 \d u \\
&= -\frac{1}{4} \int u^6 - u^8 \d u \\
&= -\frac{1}{4}\left(\frac{u^7}{7} - \frac{u^9}{9}\right) + C \\
&= -\frac{1}{4}\left(\frac{\cos^7(4\theta)}{7} - \frac{\cos^9(4\theta)}{9}\right) + C.
\end{align*}

II. We first break the $\sec^6 x$ factor into pieces, as 
	\begin{align*}
		\int \tan^{23} x \sec^6 x \d x 
		&= \int \tan^{23} x \sec^4 x \sec^2 x \d x  \\
		&= \int \tan^{23} x \left( 1 + \tan^2 x \right)^2 \sec^2 x \d x .
		\end{align*}
	Next we make the substitution $u = \tan x$, so that $\d u = \sec^2 x \d x$, and
		\begin{align*}
		\int \tan^{23} x \left( 1 + \tan^2 x \right)^2 \sec^2 x \d x
		&= \int u^{23} (1+u^2)^2 \d u  \\
		&= \int u^{23} (1 + 2u^2 + u^4) \d u  \\
		&= \int \left( u^{23} + 2u^{25} + u^{27} \right) \d u  \\
		&= \frac{1}{24} u^{24} + \frac{1}{13} u^{26} + \frac{1}{28} u^{28} + C  \\
		&= \frac{1}{24} \tan^{24} x + \frac{1}{13} \tan^{26} x + \frac{1}{28} \tan^{28} x + C.
		\end{align*}
		
III. The trick here is to recall that 
$$
\int \sec x \d x = \ln | \sec x + \tan x| + C.
$$
It follows that
\begin{align*}
		\int \tan^2 x \sec x \d x &= \int \left( \sec^2 x - 1 \right) \sec x \d x  	\\
		&= \int \sec^3 x \d x - \int \sec x \d x  	\\
		&= \int \sec^3 x \d x - \ln | \sec x + \tan x| 
		\end{align*}
	To evaluate $\int \sec^3 x \d x$, we use integration by parts with
		{
		\[
		u = \sec x 				\qquad	\d v = \sec^2 x \d x
		\]
		\[
		\d u = \sec x \tan x \d x	\qquad	v = \tan x.
		\]
		}
	So
		\begin{equation}\label{equation 2}
		\int \sec^3 x \d x = \sec x \tan x - \int \tan^2 x \sec x \d x.
		\end{equation}
	Combining our work yields
		\begin{align*}
		\int \tan^2 x \sec x \d x &= \int \sec^3 x \d x - \ln | \sec x + \tan x|   \\
		\int \tan^2 x \sec x \d x &= \sec x \tan x - \int \tan^2 x \sec x \d x - \ln | \sec x + \tan x |  \\
		2 \int \tan^2 x \sec x \d x &= \sec x \tan x - \ln | \sec x + \tan x | + C  \\
		\int \tan^2 x \sec x \d x &= \frac{1}{2} \left( \sec x \tan x - \ln | \sec x + \tan x | \right) + C.
		\end{align*}
		
		IV. We first apply trigonometric identities to conclude that
		\begin{align*}
		\int \tan^2 x \sin x \d x
		&= \int \frac{\sin^2 x}{\cos^2 x} \sin x \d x  \\
		&= \int \frac{1-\cos^2 x}{\cos^2 x} \sin x \d x.
		\end{align*}
	Now we substitute $u = \cos x $, so that $\d u = - \sin x \d x$. This gives us that
		\begin{align*}
		\int \tan^2 x \sin x \d x &= \int \frac{1-u^2}{u^2} (-1) \d u  \\
		&= \int \frac{u^2 - 1}{u^2} \d u  \\
		&= \int \left( 1 - u^{-2} \right) \d u  \\
		&= u + \frac{1}{u} + C  \\
		&= \cos x + \sec x + C.
		\end{align*}
\end{freeResponse}

\begin{problem}
Evaluate the definite integral
$$
\int_{- \pi}^0 \sqrt{1 - \cos^2 x} \d x.
$$
\end{problem}

\begin{freeResponse}
Using the Pythagorean identity, we have
\begin{align*}
		\int_{- \pi}^0 \sqrt{1 - \cos^2 x} \d x
		&= \int_{- \pi}^0 \sqrt{\sin^2 x} \d x  \\
		&= \int_{- \pi}^0 | \sin x | \d x.
		\end{align*}
	Now, when $-\pi \leq x \leq 0$, $\sin x \leq 0$.  
	Thus, on this region, $|\sin x | = - \sin x$.
	So we continue
		\begin{align*}
		\int_{- \pi}^0 \sqrt{1 - \cos^2 x} \d x
		&= \int_{- \pi}^0 - \sin x \d x  \\
		&= \eval{\cos x}_{-\pi}^0  \\
		&= \cos(0) - \cos(-\pi) = 1 - (-1) = 2.
		\end{align*}
\end{freeResponse}
\end{document}
