\documentclass[handout]{ximera}
%handout:  for handout version with no solutions or instructor notes
%handout,instructornotes:  for instructor version with just problems and notes, no solutions
%noinstructornotes:  shows only problem and solutions

%% handout
%% space
%% newpage
%% numbers
%% nooutcomes

%I added the commands here so that I would't have to keep looking them up
%\newcommand{\RR}{\mathbb R}
%\renewcommand{\d}{\,d}
%\newcommand{\dd}[2][]{\frac{d #1}{d #2}}
%\renewcommand{\l}{\ell}
%\newcommand{\ddx}{\frac{d}{dx}}
%\everymath{\displaystyle}
%\newcommand{\dfn}{\textbf}
%\newcommand{\eval}[1]{\bigg[ #1 \bigg]}

%\begin{image}
%\includegraphics[trim= 170 420 250 180]{Figure1.pdf}
%\end{image}

%add a ``.'' below when used in a specific directory.

\input{../../../preamble.tex}



\author{Tom Needham}

\outcome{Evaluate integrals using partial fraction decompositions.}

\title[]{Partial Fractions}

\begin{document}
\begin{abstract}
\end{abstract}
\maketitle

\vspace{-0.9in}

\section{Discussion Questions}

\begin{problem}
Classify each of the following expressions as an irreducible quadratic, a product of distinct linear factors, or a product of repeated linear factors.
\begin{center}
\begin{tabular}{lll}
I. $x^2+5x+1$ \hspace{.4in} II. $x^2$ \hspace{.4in} III. $x^2+x+1$
\end{tabular}
\end{center}
\end{problem}

\begin{freeResponse}
I. Although it may not be immediately obvious how to factor it, this quadratic is reducible. To test this, one checks the discriminant $b^2-4ac$; the discriminant is  $\geq 0$ if and only if the polynomial can be factored, and is strictly greater than zero if and only if the factors are distinct. In this case the discriminant is $5^2-4 \cdot 1 \cdot 1 = 21 > 0$. The expression is therefore a product of distinct linear factors.

II. This expression is a product of the repeated linear factor $x$.

III. The discriminant is $1^2-4 \cdot 1 \cdot 1 = -3 < 0$, so the quadratic is irreducible.
\end{freeResponse}

\begin{problem}
A student claims that the partial fraction decomposition for $\frac{6x^2+7x+1}{x(2x+1)^2}$ is $\frac{Ax+B}{(2x+1)^2}+\frac{C}{x}$ and justifies his or her response by finding that $A=2$, $B=3$ and $C=1$.

\begin{itemize}
\item[I.] Is it true that $\frac{6x^2+7x+1}{x(2x+1)^2}+\frac{1}{x} = \frac{2x+3}{(2x+1)^2}+\frac{1}{x}$?
\item[II.] Is this the correct partial fraction decomposition?
\end{itemize}
\end{problem}

\begin{freeResponse}
I. This is true, as we can readily check:
$$
\frac{2x+3}{(2x+1)^2}+\frac{1}{x} = \frac{2x^2+3x}{x(2x+1)^2} + \frac{(2x+1)^2}{x(2x+1)^2} = \frac{2x^2+3x+4x^2+4x+1}{x(2x+1)^2} =\frac{6x^2+7x+1}{x(2x+1)^2}.
$$

II. Remember that the whole point of the method of partial fraction decomposition is to rewrite the rational function in an equivalent way which \emph{we know how to integrate}. The student has provided an equivalent expression for the rational function, but their expression includes the term  $\frac{2x+3}{(2x+1)^2}$, and it is not clear how to find the antiderivative of this term. The correct partial fraction decomposition is of the form
$$
\frac{6x^2+7x+1}{x(2x+1)^2} = \frac{A}{x} + \frac{B}{2x+1} + \frac{C}{(2x+1)^2}.
$$
Note that each term in the resulting definition is something that we know how to integrate. 
\end{freeResponse}

\section{Group Work}

\begin{problem}
Determine the form of the partial fraction decomposition of each expression, but don't solve for constants.
\begin{center}
\begin{tabular}{lll}
I. $\frac{2x+1}{x^2+5x+6}$ \hspace{.2in} II. $\frac{2x^2+x+3}{(x^2-2x+1)(x+2)}$ \hspace{.2in} III. $\frac{3x^2+x+1}{3x^3+3x^2+6x}$
\end{tabular}
\end{center}
\end{problem}

\begin{freeResponse}
The partial fraction decompositions take the forms:

I. $\frac{2x+1}{x^2+5x+6} = \frac{2x+1}{(x+2)(x+3)} = \frac{A}{x+2} + \frac{B}{x+3}$

II. $\frac{2x^2+x+3}{(x^2-2x+1)(x+2)} = \frac{2x^2+x+3}{(x-1)^2(x+2)} = \frac{A}{x-1} + \frac{B}{(x-1)^2} + \frac{C}{x+2}$

III. $\frac{3x^2+x+1}{3x^3+3x^2+6x} = \frac{3x^2 + x + 1}{3x(x^2+x + 2)} = \frac{A}{3x} + {Bx+C}{x^2+x+2}$
\end{freeResponse}

\begin{problem}
Evaluate the integral
$$
\int \frac{1}{x^3-x^2} \d x.
$$
\end{problem}

\begin{freeResponse}
The partial fraction decomposition of the integrand is given by 
$$
\frac{1}{x^3-x^2} = \frac{1}{x^2(x-1)} = \frac{A}{x} + \frac{B}{x^2} + \frac{C}{x-1}.
$$
Clearing denominators in this equation, we have
$$
1 = Ax(x-1) + B(x-1) + Cx^2 = (A + C)x^2 + (-A + B) x + (-B).
$$
Comparing terms by degree, it must be that $-B = 1$, or $B=-1$. We also have $-A+B = 0$, or $A=B=-1$. Finally, $A+C=0$ implies $C = -A = 1$. We conclude that 
$$
\frac{1}{x^3-x^2} = -\frac{1}{x} - \frac{1}{x^2} + \frac{1}{x-1}.
$$
Therefore
\begin{align*}
\int \frac{1}{x^3-x^2} \d x &= \int \frac{1}{x^3-x^2} = \int -\frac{1}{x} - \frac{1}{x^2} + \frac{1}{x-1}\d x  \\
&= -\ln |x| + \frac{1}{x} + \ln |x-1| + C.
\end{align*} 
\end{freeResponse}

\begin{problem}
Consider the integral
$$
\int_2^3 \frac{1}{x^2-1} \d x.
$$
Evaluate the integral in two ways: first by trigonometric substitution with $x=\sec \theta$, then via partial fraction decomposition. For the trigonometric substitution method, it may be useful to recall that
$$
\int \csc \theta \d \theta = -\ln | \csc \theta + \cot \theta | + C.
$$
If we change the bounds of integration to $x=0$ to $x=1/2$, would both methods still be valid?
\end{problem}

\begin{freeResponse}
First let $x=\sec \theta$, so that $\d x = \sec \theta \tan \theta \d \theta$. Then
\begin{align*}
\int \frac{1}{x^2-1} \d x &= \int \frac{1}{\tan^2 \theta} \sec \theta \tan \theta \d \theta \\
&= \int \frac{\sec \theta}{\tan \theta} \d \theta \\
&= \int \frac{1}{\cos \theta} \frac{\cos \theta}{\sin \theta} \d \theta \\
&= \int \csc \theta \d \theta \\
&= \ln |\csc \theta - \cot \theta| + C \\
&= \ln \left|\frac{x}{\sqrt{x^2-1}} - \frac{1}{\sqrt{x^2-1}}\right|+C,
\end{align*}
with the last line derived via a reference triangle. Therefore
\begin{align*}
\int_2^3 \frac{1}{x^2-1} \d x &= \eval{\ln \left|\frac{x}{\sqrt{x^2-1}} - \frac{1}{\sqrt{x^2-1}}\right|}_2^3 \\
&= \ln \left|\frac{3}{\sqrt{8}} - \frac{1}{\sqrt{8}}\right| - \ln \left| \frac{2}{\sqrt{3}} - \frac{1}{\sqrt{3}}\right|\\
&= \ln \frac{1}{\sqrt{2}} - \ln \frac{1}{\sqrt{3}} \\
&= -\frac{1}{2} \ln 2 + \frac{1}{2} \ln 3.
\end{align*}

On the other hand, the partial fraction decomposition of the integrand is 
$$
\frac{1}{x^2-1} = \frac{1}{(x+1)(x-1)} = \frac{A}{x+1} + \frac{B}{x-1}.
$$
Clearing denominators, we have
$$
1 = A(x-1) + B(x+1) = (A+B)x + (-A+B).
$$
Comparing terms of the same degree, we have $-A+B=1$ and $A+B = 0$. Solving the second equation yields $A=-B$, and substituting this into the first equation yields $2B=1$, or $B=1/2$. Therefore $A=-1/2$, and 
$$
\frac{1}{x^2-1} = -\frac{1/2}{x+1} + \frac{1/2}{x-1}.
$$
The integral is therefore given by
\begin{align*}
\int_2^3 \frac{1}{x^2-1} \d x &= \int_2^3  -\frac{1/2}{x+1} + \frac{1/2}{x-1} \d x \\
&= \eval{-\frac{1}{2} \ln |x+1| + \frac{1}{2} \ln |x-1| }_2^3 \\
&= \frac{1}{2}\left(- \ln 4 + \ln 2 + \ln 3 - \ln 1\right) \\
&=  -\frac{1}{2} \ln 2 + \frac{1}{2} \ln 3.
\end{align*}
We therefore obtain the same answer as we did using trigonometric substitution, but with a smaller amount of effort. Moreover, making the substitution $x=\sec \theta$ implicitly assumes that $|x| \geq 1$ (since this is the range of the secant function). This means that the trigonometric substitution method would not be valid if we integrated over any region containing $x$ with $|x| < 1$. 
\end{freeResponse}


\end{document}
